election WIP

examples/Messaging/Election.v
@@ -230,7 +230,7 @@ Definition max_id n ids (wf : ids_wf n ids) : nat.
 Admitted.
 
 Lemma max_id_correct : forall n ids (wf : ids_wf n ids),
-  forall k, k <> max_id wf -> List.nth k ids 0 < List.nth (max_id wf) ids 0.
+  max_id wf < n /\ forall k, k <> max_id wf -> List.nth k ids 0 < List.nth (max_id wf) ids 0.
 Admitted.
 
 Section Election.
@@ -238,8 +238,12 @@ Section Election.
 Context {n : nat} (Hn : n <> 0) (ids : list nat) (ids_wf : ids_wf n ids).
 
 Let im := max_id ids_wf.
-Let max := List.nth im ids 0.
 Let pid i := List.nth i ids 0.
+Let max := pid im.
+
+Lemma pid_inj : forall i j (Hi : i < n) (Hj : j < n), pid i = pid j -> i = j.
+Proof.
+Admitted.
 
 Variant message :=
   | Candidate (u: nat)
@@ -324,43 +328,46 @@ Context (Hc : sched_correct sched next_id).
 
 Open Scope nat_scope.
 
-Definition from_to_ (i j : nat) : nat -> Prop :=
-  fun k => i <= k /\ k < j.
-
 Definition from_to (i j : nat) : nat -> Prop :=
   fun k =>
-    (i <= j -> from_to_ i j k) /\
-    (j < i -> from_to_ j n k /\ from_to_ 0 i k).
+    (i <= j -> i <= k < j) /\
+    (j < i -> i <= k < n \/ 0 <= k < j).
 
 Lemma from_to_bound : forall (i j k : nat) (Hi: i < n) (Hj: j < n), from_to i j k ->
   k < n.
 Proof.
-  intros. destruct H. unfold from_to_ in *. lia.
+  intros. destruct H. lia.
 Qed.
 
-Lemma from_to__dec : forall (i j k : nat), { from_to_ i j k } + { ~from_to_ i j k }.
+Lemma from_to_dec_ : forall (i j k : nat), { i <= j < k } + { ~i <= j < k }.
 Proof.
-  intros. unfold from_to_.
-  destruct (Compare_dec.le_dec i k).
+  intros.
+  destruct (Compare_dec.le_dec i j).
   2: tauto.
-  destruct (Compare_dec.lt_dec k j); tauto.
+  destruct (Compare_dec.lt_dec j k); tauto.
 Qed.
 
 Lemma from_to_dec : forall (i j k : nat), { from_to i j k } + { ~from_to i j k }.
 Proof.
-  intros. unfold from_to. Locate "<=". Search nat le sumbool.
+  intros. unfold from_to.
   destruct (Compare_dec.le_lt_dec i j).
-  - destruct (from_to__dec i j k); [| tauto].
+  - destruct (from_to_dec_ i k j); [| tauto].
     left. split; [tauto | lia].
-  - destruct (from_to__dec j n k); [| tauto].
-    destruct (from_to__dec 0 i k); [| tauto].
-    left. split; [lia | tauto].
+  - destruct (from_to_dec_ i k n); [left; lia |].
+    destruct (from_to_dec_ 0 k j); [left; lia |].
+    right. lia.
 Qed.
 
 Definition next_proc_and_msg st :=
   match st.(s_progress) with
   | MaxCandidate d => ((im + d) mod n, Candidate max)
   | MaxElected d => ((im + d + 1) mod n, Elected max)
+  end.
+
+Definition noop_msg i msg :=
+  match msg with
+  | Candidate c => Nat.ltb c (pid i)
+  | Elected e => false
   end.
 
 Definition next_proc st :=
@@ -402,7 +409,7 @@ Definition handle_election_state (qs: list (list message)) (st: election_state) 
     end
   | Recv i =>
     let s := match hd_error (nth i qs []%list) with
-    | Some m => ProcProcessing m
+    | Some m => if noop_msg i m then ProcWaiting else ProcProcessing m
     | None => ProcWaiting
     end in
     mk_election_state (nth_map (fun _ => s) st.(s_procs) i) st.(s_progress)
@@ -431,21 +438,23 @@ Definition election_invariant_candidates
   st qs :=
   (* Well-formedness *)
   let procs := st.(s_procs) in
-  (forall i, count_occ eq_dec_message (concat (ext_mailbox qs st)) (Candidate i) <= 1) /\
+  (forall msg, count_occ eq_dec_message (concat (ext_mailbox qs st)) msg <= 1) /\
   (forall i j, In (Candidate i) (List.nth j (ext_mailbox qs st) []%list) -> exists k, k < n /\ i = List.nth k ids 0) /\
   forall i (Hi : (i < n)%nat),
-    match List.nth_error procs i with
-    | Some ProcBegin => ~ In (Candidate i) (concat (ext_mailbox qs st))
+    match List.nth i procs ProcBegin with
+    | ProcBegin => ~ In (Candidate i) (concat (ext_mailbox qs st))
     | _ =>
       (* A losing candidate cannot travel beyond the process with the max id *)
-      (forall k, k <> im -> In (Candidate (List.nth i ids 0)) (List.nth k (ext_mailbox qs st) []%list) -> from_to ((i + 1) mod n) ((im + 1) mod n) k)
+      (forall k, k <> im -> In (Candidate (pid i)) (List.nth k (ext_mailbox qs st) []%list) -> from_to ((i + 1) mod n) ((im + 1) mod n) k)
     end.
 
 (* Invariant regarding the position in the mailbox of the current message of interest *)
 Definition election_invariant_msg_location
   (st : election_state) (qs: list (list message)) (i: nat) (m: message) :=
   snd st.(s_queue) = match List.nth i st.(s_procs) ProcBegin with ProcProcessing m => true | _ => false end /\
-  forall j k, List.nth_error (List.nth j (ext_mailbox qs st) []%list) k = Some m <-> j = i /\ k = fst st.(s_queue).
+  (forall j k, List.nth_error (List.nth j (ext_mailbox qs st) []%list) k = Some m <->
+    j = i /\ k = fst st.(s_queue) - match List.nth i st.(s_procs) ProcBegin with ProcBegin => 1 | _ => 0 end) /\
+  match List.nth i st.(s_procs) ProcBegin with ProcBegin => fst st.(s_queue) > 0 | _ => True end.
 
 (* Invariant regarding the max candidate *)
 Definition election_invariant_max
@@ -455,7 +464,7 @@ Definition election_invariant_max
   match elected_progress with
   | MaxCandidate d =>
     (* The leader has not been elected yet *)
-    (forall c, ~In (Elected c) (concat (ext_mailbox qs st))) /\
+    (forall c k, ~In (Elected c) (List.nth k (ext_mailbox qs st) []%list)) /\
     {Hd : d <= n |
       (* The message can only be in the mailbox at distance d from the max *)
       (d <> 0 -> election_invariant_msg_location st qs ((im + d) mod n) (Candidate max)) /\
@@ -481,10 +490,10 @@ Definition election_state_invariant st qs :=
 (* Ties the proc_states to the ctrees *)
 Definition election_src_invariant_candidate st i (t : ctree (netE message) B01 unit) :=
   match st with
-  | ProcBegin => t ≅ proc i n
+  | ProcBegin => t ≅ proc i ((i + 1) mod n)
   | ProcWaiting =>
     (t ≅ proc_loop i ((i + 1) mod n))
-  | ProcProcessing m => t ≅ proc_loop_handle_msg i ((i + 1) mod n) (Some m)
+  | ProcProcessing m => t ≅ proc_loop_handle_msg i ((i + 1) mod n) (Some m) /\ noop_msg i m = false
   | ProcElected => t ≅ Ret tt \/ t ≅ stuckD
   end.
 
@@ -492,8 +501,9 @@ Definition election_src_invariant_candidate st i (t : ctree (netE message) B01 u
 Definition election_src_invariant st (v : vec n (ctree (netE message) B01 unit)) :=
   match st.(s_progress) with
   | MaxCandidate d =>
-    (d = 0 -> nth im st.(s_procs) ProcBegin = ProcBegin) /\
-    forall k, nth k st.(s_procs) ProcBegin <> ProcElected
+    (d = 0 <-> nth im st.(s_procs) ProcBegin = ProcBegin) /\
+    (forall k, nth k st.(s_procs) ProcBegin <> ProcElected) /\
+    (forall k, (from_to im ((im + d) mod n) k \/ d = n) -> nth k st.(s_procs) ProcBegin <> ProcBegin)
   | MaxElected d =>
     forall i (Hi: i < n),
     nth i st.(s_procs) ProcBegin <> ProcBegin /\
@@ -511,6 +521,28 @@ Record election_invariant v qs st :=
     election_src_invariant_candidate (nth i st.(s_procs) ProcBegin) i v[@Fin.of_nat_lt Hi];
   wf_src_progress : election_src_invariant st v
 }.
+
+(*Lemma election_candidates_proc_states :
+  forall v qs st d,
+  election_invariant v qs st ->
+  st.(s_progress) = MaxCandidate d ->
+  forall i (Hi : i < n),
+  (nth i st.(s_procs) ProcBegin = ProcWaiting) \/
+  (exists m, nth i st.(s_procs) ProcBegin = ProcProcessing m) \/
+  (d <> n /\ ~from_to (im mod n) ((im + d) mod n) i /\
+    (nth i st.(s_procs) ProcBegin = ProcBegin)).
+Proof.
+  intros.
+  apply wf_src_progress in H. red in H. rewrite H0 in H.
+  destruct (nth i st.(s_procs) ProcBegin) eqn:?.
+  - right. right.
+  destruct (from_to_dec (S im mod n) ((im + d + 1) mod n) i).
+  - left. split; auto.
+    now apply H in f.
+  - right. split; auto.
+    apply H in Hi as [? ?]. apply not_iff_compat in H2. apply H2 in n0.
+    destruct (nth i (s_procs st) ProcBegin) eqn:?; eauto with exfalso.
+Qed.*)
 
 Lemma election_elected_proc_states :
   forall v qs st d,
@@ -545,7 +577,7 @@ Qed.
  *)
 Definition election_variant (st : election_state) : nat * (nat * nat) :=
   match st.(s_progress) with
-  | MaxCandidate d => (n + n + 1 - d, (fst st.(s_queue), if snd st.(s_queue) then 0 else 1))
+  | MaxCandidate d => (n + n - d, (fst st.(s_queue), if snd st.(s_queue) then 0 else 1))
   | MaxElected d => (n - d - 1, (fst st.(s_queue), if snd st.(s_queue) then 0 else 1))
   end.
 
@@ -583,7 +615,7 @@ Lemma election_other_messages :
   election_invariant v qs st ->
   k <> next_proc st ->
   In msg (List.nth k (ext_mailbox qs st) []%list) ->
-  exists i, i <> im /\ msg = Candidate (List.nth i ids 0).
+  exists i, i < n /\ i <> im /\ msg = Candidate (List.nth i ids 0).
 Proof.
   intros. destruct H. destruct wf_progress0.
   destruct (s_progress st) eqn:?.
@@ -592,19 +624,16 @@ Proof.
     assert (k < length (ext_mailbox qs st)).
     { eapply nth_not_default. eapply in_not_nil. apply H1. }
     destruct msg.
-    2: {
-      exfalso. apply (H2 u). apply in_concat. eexists. split; [| apply H1].
-      now apply nth_In.
-    }
+    2: { exfalso. now apply (H2 u k). }
     destruct wf_candidates0 as (_ & ? & _).
     apply H4 in H1 as ?. destruct H5 as (? & ? & ->).
-    exists x0. split; auto. intro. subst.
+    exists x0. split; auto. split; auto. intro. subst.
     destruct (nat_eqdec n0 0).
     + apply a in e. apply e.
       apply in_concat. eexists. split; [| apply H1].
       now apply nth_In.
     + apply a in n1. destruct n1 as [_ ?].
-      apply In_nth_error in H1 as []. apply H6 in H1 as [-> ->].
+      apply In_nth_error in H1 as []. apply H6 in H1 as [-> _].
       unfold next_proc, next_proc_and_msg in H0. rewrite Heqe in H0. contradiction.
   - (* phase 2 *)
     destruct H2 as (? & ? & ?).
@@ -612,11 +641,11 @@ Proof.
     { eapply nth_not_default. eapply in_not_nil. apply H1. }
     destruct msg.
     + destruct wf_candidates0 as (_ & ? & _). apply H5 in H1 as ?. destruct H6 as (? & ? & ->).
-      exists x0. split; auto. intro. subst.
+      exists x0. split; auto. split; auto. intro. subst.
       now apply H2 in H1.
     + exfalso. destruct (nat_eqdec u max). subst.
-      * destruct H3 as [ [_ ?] _]. red in H3.
-        apply In_nth_error in H1 as []. apply H3 in H1 as [-> ->].
+      * destruct H3 as [ [_ ?] _].
+        apply In_nth_error in H1 as []. apply H3 in H1 as [-> _].
         unfold next_proc, next_proc_and_msg in H0. rewrite Heqe in H0. contradiction.
       * now apply H3 in H1.
 Qed.
@@ -642,13 +671,98 @@ Qed.
 
 (* ktrans inversion lemmas for leader election processes *)
 
+Lemma ktrans_proc_begin_inv : forall i (Hi : i < n) t' v qs qs' st st' (INV: election_invariant v qs st),
+  i <> next_proc st ->
+  nth i st.(s_procs) ProcBegin = ProcBegin ->
+  ktrans (v[@Fin.of_nat_lt Hi], (qs, st)) (t', (qs', st')) ->
+  t' ≅ proc_loop i ((i + 1) mod n) /\
+  qs' = nth_map (fun q => (q ++ [Candidate (pid i)])%list) qs ((i + 1) mod n) /\
+  st' = mk_election_state
+    (nth_map (fun _ => ProcWaiting) st.(s_procs) i)
+    st.(s_progress)
+    st.(s_queue).
+Proof.
+  intros. apply election_map_proc_state with (Hi := Hi) in INV as ?.
+  red in H2. rewrite H0 in H2.
+  unfold proc in H2. setoid_rewrite bind_trigger in H2.
+  rewrite H2 in H1. apply ktrans_vis_inv in H1 as (? & ? & -> & ?).
+  injection H3 as -> ->.
+  split; auto. split; auto.
+  destruct st.(s_progress) eqn:?.
+  - destruct (Nat.eq_dec i im).
+    + subst. rewrite Nat.eqb_refl.
+      apply wf_src_progress in INV. red in INV. rewrite Heqe in INV.
+      apply (proj1 INV) in H0. subst.
+      unfold next_proc, next_proc_and_msg in H. rewrite Heqe in H.
+      exfalso. apply H.
+      rewrite Nat.mod_small; [| lia]. cbn. lia.
+    + apply ids_wf in n1. apply Nat.eqb_neq in H, n1. rewrite H.
+      unfold max, pid. rewrite n1. reflexivity. 
+  - apply wf_src_progress in INV as ?. red in H3. rewrite Heqe in H3.
+    now apply H3 in H0.
+Qed.
+
+Lemma ktrans_proc_begin_next_inv : forall i (Hi : i < n) t' v qs qs' st st' (INV: election_invariant v qs st),
+  i = next_proc st ->
+  nth i st.(s_procs) ProcBegin = ProcBegin ->
+  ktrans (v[@Fin.of_nat_lt Hi], (qs, st)) (t', (qs', st')) ->
+  t' ≅ proc_loop i ((i + 1) mod n) /\
+  qs' = nth_map (fun q => (q ++ [Candidate (pid i)])%list) qs ((i + 1) mod n) /\
+  st' = mk_election_state
+    (nth_map (fun _ => ProcWaiting) st.(s_procs) i)
+    (if pid i =? max then MaxCandidate 1 else st.(s_progress))
+    (handle_send qs st i st.(s_queue)).
+Proof.
+  intros. apply election_map_proc_state with (Hi := Hi) in INV as ?.
+  red in H2. rewrite H0 in H2.
+  unfold proc in H2. setoid_rewrite bind_trigger in H2.
+  rewrite H2 in H1. apply ktrans_vis_inv in H1 as (? & ? & -> & ?).
+  injection H3 as -> ->.
+  split; auto. split; auto.
+  destruct st.(s_progress) eqn:?.
+  - destruct (Nat.eq_dec i im).
+    + subst. rewrite Nat.eqb_refl.
+      apply wf_src_progress in INV. red in INV. rewrite Heqe in INV.
+      rewrite e in H0. apply (proj1 INV) in H0. subst. reflexivity.
+    + apply ids_wf in n1. apply Nat.eqb_neq in n1.
+      unfold max, pid. rewrite n1. subst. rewrite Nat.eqb_refl.
+      reflexivity.
+  - apply wf_src_progress in INV as ?. red in H3. rewrite Heqe in H3.
+    now apply H3 in H0.
+Qed.
+
 Lemma ktrans_proc_loop_some_inv : forall i j t' qs qs' st st' m,
   ktrans ((proc_loop i j), (qs, st)) (t', (qs', st')) ->
   List.hd_error (List.nth i qs []%list) = Some m ->
+  noop_msg i m = false ->
   t' ≅ proc_loop_handle_msg i j (Some m) /\
   qs' = nth_map (fun _ => tl (List.nth i qs []%list)) qs i /\
   st' = mk_election_state
     (nth_map (fun _ => ProcProcessing m) st.(s_procs) i)
+    st.(s_progress)
+    (if i =? next_proc st then handle_recv st.(s_queue) else st.(s_queue)).
+Proof.
+  intros.
+  unfold proc_loop in H. rewrite unfold_iter in H.
+  rewrite bind_bind in H. setoid_rewrite bind_trigger in H.
+  apply ktrans_vis_inv in H as (? & ? & ? & ?).
+  cbn in H3. unfold execState in H3. cbn in H2, H3.
+  destruct (nth i qs []%list) eqn:?. { discriminate. }
+  inv H0.
+  inversion H3. cbn. split; [| split; [auto |] ].
+  2: now destruct (noop_msg i m).
+  cbn in H. unfold proc_loop_handle_msg, proc_handle_msg.
+  rewrite H. upto_bind_eq. destruct x1 as [ [] | [] ]; reflexivity.
+Qed.
+
+Lemma ktrans_proc_loop_some_noop_inv : forall i j t' qs qs' st st' m,
+  ktrans ((proc_loop i j), (qs, st)) (t', (qs', st')) ->
+  List.hd_error (List.nth i qs []%list) = Some m ->
+  noop_msg i m = true ->
+  t' ≅ Guard (proc_loop i j) /\
+  qs' = nth_map (fun _ => tl (List.nth i qs []%list)) qs i /\
+  st' = mk_election_state
+    (nth_map (fun _ => ProcWaiting) st.(s_procs) i)
     st.(s_progress)
     (if i =? next_proc st then handle_recv (s_queue st) else s_queue st).
 Proof.
@@ -656,12 +770,15 @@ Proof.
   unfold proc_loop in H. rewrite unfold_iter in H.
   rewrite bind_bind in H. setoid_rewrite bind_trigger in H.
   apply ktrans_vis_inv in H as (? & ? & ? & ?).
-  cbn in H2. unfold execState in H2. cbn in H1, H2.
+  cbn in H3. unfold execState in H3. cbn in H2, H3.
   destruct (nth i qs []%list) eqn:?. { discriminate. }
   inv H0.
-  inversion H2. cbn. intuition.
+  inversion H3. cbn. split; [| split; [auto |] ].
+  2: now destruct (noop_msg i m).
+  unfold noop_msg in H1. destruct m; [| discriminate].
+  apply Nat.ltb_lt, Nat.compare_lt_iff in H1.
   cbn in H. unfold proc_loop_handle_msg, proc_handle_msg.
-  rewrite H. upto_bind_eq. destruct x1 as [ [] | [] ]; reflexivity.
+  rewrite H. rewrite H1. rewrite bind_ret_l. reflexivity.
 Qed.
 
 Lemma ktrans_proc_loop_none_inv : forall i j t' qs qs' st st',
@@ -677,7 +794,7 @@ Proof.
   apply ktrans_vis_inv in H as (? & ? & ? & ?).
   cbn in H2. unfold execState in H2. cbn in H1, H2.
   destruct (nth i qs []%list) eqn:?. 2: discriminate.
-  cbn in H1, H2. inv H2. intuition.
+  cbn in H1, H2. inv H2. split; auto.
   rewrite H. cbn. rewrite bind_ret_l. now apply br_equ.
 Qed.
 
@@ -708,27 +825,55 @@ Qed.
 Lemma proc_handle_msg_inv : forall i (Hi : i < n) j msg v qs st
   (INV: election_invariant v qs st),
   v[@Fin.of_nat_lt Hi] ≅ proc_loop_handle_msg i j (Some msg) ->
-  exists msg', List.nth i st.(s_procs) ProcBegin = ProcProcessing msg' /\
-  (msg' = msg) \/
+  exists msg', List.nth i st.(s_procs) ProcBegin = ProcProcessing msg' /\ (
+    (noop_msg i msg' = false /\ msg' = msg) \/
     (exists c c', msg = Candidate c /\ msg' = Candidate c' /\ c < pid i /\ c' < pid i) \/
     (msg = Candidate (pid i) /\ msg' = Elected (pid i)) \/
-    (msg = Elected (pid i) /\ msg' = Candidate (pid i)).
+    (msg = Elected (pid i) /\ msg' = Candidate (pid i))).
 Proof.
   intros.
   pose proof INV.(wf_src_candidates). red in H0. specialize (H0 i Hi).
   unfold proc, proc_loop_handle_msg, proc_loop, proc_handle_msg, send, recv in *.
-  destruct (nth i (s_procs st) ProcBegin) eqn:?; [| | | destruct H0]; rewrite H0 in H; clear H0.
+  destruct (nth i (s_procs st) ProcBegin) eqn:?; [| | destruct H0 as [H0 _] | destruct H0]; rewrite H0 in H; clear H0.
   - destruct msg; try solve [inv_equ].
     destruct (u ?= pid i) eqn:?; inv_equ.
     inv EQe. apply Nat.compare_gt_iff in Heqc. lia.
   - rewrite unfold_iter, bind_bind in H. destruct msg; try solve [inv_equ].
     destruct (u ?= pid i) eqn:?; inv_equ.
-  - apply proc_handle_msg_equ_inv in H; auto. intuition; eauto 6.
-    destruct H as (? & ? & ? & ? & ? & ?). eauto 9.
+  - apply proc_handle_msg_equ_inv in H; auto. intuition; eauto 7.
+    + eapply wf_src_candidates with (Hi := Hi) in INV. red in INV. rewrite Heqp in INV.
+      destruct INV. eauto.
+    + destruct H as (? & ? & ? & ? & ? & ?). eauto 10.
   - destruct msg; try solve [inv_equ].
     destruct (u ?= pid i) eqn:?; inv_equ.
   - destruct msg; try solve [inv_equ].
     destruct (u ?= pid i) eqn:?; inv_equ.
+Qed.
+
+Lemma election_no_other_elected : forall v qs st (INV: election_invariant v qs st),
+  forall i j, j <> max -> ~ In (Elected j) (nth i (ext_mailbox qs st) []%list).
+Proof.
+  intros. apply wf_progress in INV. red in INV. destruct st.(s_progress).
+  - destruct INV as (_ & ? & _). auto.
+  - destruct INV as (_ & _ & _ & _ & ?). auto.
+Qed.
+
+Lemma proc_handle_msg_candidate_nonmax_inv : forall i (Hi : i < n) j c v qs st
+  (INV: election_invariant v qs st),
+  i <> im ->
+  v[@Fin.of_nat_lt Hi] ≅ proc_loop_handle_msg i j (Some (Candidate c)) ->
+  exists msg', List.nth i st.(s_procs) ProcBegin = ProcProcessing msg' /\ (
+    (noop_msg i msg' = false /\ msg' = Candidate c) \/
+    (exists c', msg' = Candidate c' /\ c < pid i /\ c' < pid i)).
+Proof.
+  intros. eapply proc_handle_msg_inv in H0; eauto.
+  destruct H0 as (? & ? & [ [] | [] ]).
+  - eauto.
+  - destruct H1 as (? & ? & ? & -> & ? & ?). injection H1 as <-. eauto 7.
+  - destruct H1 as [ [? ->] | [] ]; [| discriminate].
+    injection H1 as ->.
+    eapply election_processing_ext_mailbox in H0; eauto. apply hd_error_in in H0.
+    eapply election_no_other_elected in H0; eauto. destruct H0. now apply ids_wf.
 Qed.
 
 Lemma ktrans_proc_handle_other_candidate_gt_inv : forall i (Hi : i < n) j c t' v qs qs' st st'
@@ -752,17 +897,263 @@ Proof.
   cbn in H2. unfold execState in H2. cbn in H2.
   injection H2 as ?. subst. split; auto.
   apply Nat.eqb_neq in H1. rewrite !H1.
-  eapply proc_handle_msg_inv in Hvi as ?; eauto. destruct H2 as [? [? | [? | [? | ?] ] ] ].
-  2: { destruct H2 as (? & ? & ? & ? & ? & ?). apply Nat.compare_gt_iff in H0. inversion H2. lia. }
-  2, 3: destruct H2; inversion H2; apply Nat.compare_gt_iff in H0; lia.
-  destruct H2 as [? ->].
+  eapply proc_handle_msg_inv in Hvi as ?; eauto. destruct H2 as (? & ? & [? | [? | [? | ?] ] ]).
+  2: { destruct H3 as (? & ? & ? & ? & ?). apply Nat.compare_gt_iff in H0. inversion H3. lia. }
+  2, 3: destruct H3; inversion H3; apply Nat.compare_gt_iff in H0; lia.
+  destruct H3 as (? & ->).
   eapply election_processing_ext_mailbox in H2; eauto. apply hd_error_in in H2.
   apply wf_progress in INV. destruct INV. destruct st.(s_progress) eqn:?; auto.
   destruct (c =? max) eqn:?; auto. apply Nat.eqb_eq in Heqb as ->.
-  destruct H4. now apply a in H2.
+  destruct H5. now apply a in H2.
 Qed.
 
+Lemma from_succ_absurd : forall i k, i < n -> k < n -> ~from_to ((k + 1) mod n) i k.
+Proof.
+  intros * Hi Hk ?. unfold from_to in H. destruct H.
+  destruct (Nat.eq_dec k (n - 1)).
+  ++rewrite e in *. assert ((n - 1 + 1) = n) by lia. rewrite H1 in *.
+    rewrite Nat.Div0.mod_same in *.
+    pose proof (Nat.mod_upper_bound (im + 1) n). lia.
+  ++assert (k + 1 < n) by lia. apply Nat.mod_small in H1. rewrite H1 in *. lia.
+Qed.
+
+Lemma nth_neq : forall {A} (l : list A) i j d,
+  nth i l d <> nth j l d -> i <> j.
+Proof.
+  intros * ? ?. now subst.
+Qed.
+
+Lemma next_proc_bound : forall st, next_proc st < n.
+Proof.
+  intros. unfold next_proc, next_proc_and_msg.
+  destruct st.(s_progress); now apply Nat.mod_upper_bound.
+Qed.
+
+Lemma proc_begin_empty_queue : forall v qs st (INV : election_invariant v qs st),
+  nth (next_proc st) st.(s_procs) ProcBegin = ProcBegin ->
+  fst st.(s_queue) = 0 ->
+  next_proc st = im.
+Proof.
+  intros.
+  pose proof INV.(wf_progress) as [_ ?].
+  pose proof INV.(wf_src_progress). red in H2.
+  unfold next_proc, next_proc_and_msg.
+  destruct st.(s_progress) eqn:?.
+  2: { apply H2 in H; [easy |]. apply next_proc_bound. }
+  destruct H1 as (_ & ? & ? & ?).
+  destruct (Nat.eq_dec n0 0).
+  - subst. cbn. rewrite Nat.add_0_r. rewrite Nat.mod_small; [reflexivity |].
+    apply max_id_correct.
+  - exfalso. clear H3. specialize (H1 n1). destruct H1 as (_ & _ & ?).
+    unfold next_proc, next_proc_and_msg in H. rewrite Heqe in H.
+    cbn in H. rewrite H in H1. lia.
+Qed.
+
+Lemma nth_error_hd_error : forall {A} (l : list A), nth_error l 0 = hd_error l.
+Proof.
+  intros. now destruct l.
+Qed.
+
+Lemma next_msg_begin : forall v qs st (INV : election_invariant v qs st),
+  fst st.(s_queue) = 0 ->
+  st.(s_progress) = MaxCandidate 0 ->
+  List.nth (next_proc st) st.(s_procs) ProcBegin = ProcBegin.
+Proof.
+  intros.
+  pose proof INV.(wf_src_progress). red in H1.
+  unfold next_proc, next_proc_and_msg. rewrite H0 in H1 |- *.
+  assert ((im + 0) mod n = im). { rewrite Nat.add_0_r. apply Nat.mod_small. apply max_id_correct. }
+  rewrite H2. now apply H1.
+Qed.
+
+Lemma next_msg_head : forall v qs st (INV : election_invariant v qs st),
+  fst st.(s_queue) = 0 ->
+  st.(s_progress) <> MaxCandidate 0 ->
+  hd_error (List.nth (next_proc st) (ext_mailbox qs st) []%list) = Some (snd (next_proc_and_msg st)).
+Proof.
+  intros.
+  pose proof INV.(wf_progress). red in H1.
+  unfold next_proc, next_proc_and_msg in H.
+  destruct st.(s_progress) eqn:?.
+  - destruct H1 as (_ & _ & _ & ? & _).
+    assert (n0 <> 0). { intro. subst. now apply H0. }
+    specialize (H1 H2). destruct H1 as (? & ? & ?).
+    specialize (H3 ((im + n0) mod n) (fst st.(s_queue))).
+    lapply (proj2 H3).
+    2: {
+      split; auto.
+      destruct (nth ((im + n0) mod n) (s_procs st) ProcBegin) eqn:?; lia.
+    }
+    clear H3. intro. rewrite H in H3. rewrite nth_error_hd_error in H3.
+    unfold next_proc, next_proc_and_msg. now rewrite Heqe.
+  - destruct H1 as (_ & _ & _ & ? & _).
+    destruct H1 as (? & ? & ?).
+    specialize (H2 ((im + n0 + 1) mod n) (fst (s_queue st))).
+    lapply (proj2 H2).
+    2: {
+      split; auto.
+      destruct (nth ((im + n0 + 1) mod n) (s_procs st) ProcBegin) eqn:?; lia.
+    }
+    clear H2. intro. rewrite H in H2. rewrite nth_error_hd_error in H2.
+    unfold next_proc, next_proc_and_msg. now rewrite Heqe.
+Qed.
+
+Theorem election_dec_candidates :
+  forall i (Hi : i <> 0 /\ i <= n) v T st st' qs qs',
+  election_invariant v qs st ->
+  fst (election_variant st) = n + i ->
+  proj1_sig (Fin.to_nat (next_id v)) = (im + (n - i)) mod n ->
+  ktrans (sched v, (qs, st)) (T, (qs', st')) -> lt_election_variant (election_variant st') (election_variant st).
+Proof.
+  intros.
+  destruct st as [? [] ]; cbn in H0.
+  2: { destruct H. destruct wf_progress0 as (_ & _ & [? _]). lia. }
+  assert (n0 = n - i) by lia. subst. clear H0.
+  unshelve eapply election_does_progress in H as ?; eauto.
+  2: { cbn. intro. injection H0 as ?. lia. }
+  destruct H0 as (? & ? & ?).
+  eapply sched_correct_ktrans in H2 as ?; eauto. destruct H3 as (? & ? & ?). subs.
+  apply election_map_proc_state with (Hi := proj2_sig (Fin.to_nat (next_id v))) in H as ?. red in H4. cbn in H4.
+  destruct (nth (proj1_sig (Fin.to_nat (next_id v))) s_procs0 ProcBegin) eqn:?.
+  - (* ProcBegin *)
+    eapply ktrans_proc_begin_next_inv with (Hi := proj2_sig (Fin.to_nat (next_id v))) in H as ?.
+    3: eauto.
+    3: rewrite Fin.of_nat_to_nat_inv; apply H3.
+    2: { cbn. rewrite H1. apply Nat.mod_wd; auto. }
+    destruct H5 as (? & -> & ->). cbn.
+    destruct (pid (proj1_sig (Fin.to_nat (next_id v))) =? max) eqn:?.
+    + cbn. apply Nat.eqb_eq in Heqb. apply pid_inj in Heqb; [| apply (proj2_sig (Fin.to_nat _)) | apply max_id_correct].
+      rewrite Heqb in Heqp.
+      apply wf_src_progress in H. cbn in H. apply (proj1 H) in Heqp. subst. left. lia.
+    + apply Nat.eqb_neq in Heqb. apply nth_neq in Heqb.
+      right. left. cbn. unfold handle_send.
+      destruct (Nat.eq_dec (fst s_queue0) 0).
+      * rewrite e in *. exfalso.
+        eapply proc_begin_empty_queue in H as ?; auto.
+        2: { cbn. now rewrite H1 in Heqp. }
+        cbn in H6. rewrite H1 in Heqb. apply Heqb. rewrite <- H6. apply Nat.mod_wd; auto.
+      * destruct (fst s_queue0) eqn:?; [easy |].
+        cbn. lia.
+  - (* ProcWaiting *)
+    rewrite Fin.of_nat_to_nat_inv in H4. rewrite H4 in H3.
+    destruct (List.hd_error (List.nth (proj1_sig (Fin.to_nat (next_id v))) qs []%list)) eqn:?.
+    (* empty mailbox *)
+    2: {
+      apply ktrans_proc_loop_none_inv in H3 as (? & -> & ->); auto.
+      exfalso.
+    }
+    (* non-empty mailbox *)
+    destruct (noop_msg (proj1_sig (Fin.to_nat (next_id v))) m) eqn:?.
+    + apply ktrans_proc_loop_some_noop_inv with (m := m) in H3 as (? & -> & ->); auto.
+      cbn. right.
+      rewrite ((proj2 (Nat.eqb_eq _ _)) H1).
+      unfold handle_recv. cbn.
+      destruct (snd s_queue0). 2: right; left.
+      left.
+      apply wf_progress in H as ?. destruct H5 as [_ ?]. cbn in H5. destruct H5 as (_ & _ & ? & ?).
+      destruct (Nat.eq_dec (n - i) 0).
+      * assert (n = i) by lia. subst. clear e.
+        destruct (Nat.eq_dec (fst s_queue0) 0); [| lia].
+        exfalso. apply next_msg_begin in H as ?; auto. 2: cbn; f_equal; lia.
+        cbn in H7. assert ((im + (n - n)) = im) by lia.
+        rewrite <- H1 in H7. rewrite H7 in Heqp. discriminate.
+      * specialize (H5 n0).
+        destruct (Nat.eq_dec (fst s_queue0) 0); [| lia].
+        apply next_msg_head in H as ?; auto.
+        2: { intro. now injection H7. }
+        cbn in H7. unfold ext_mailbox in H7. cbn in H7.
+        change []%list with (ext_mailbox1 ([]%list, ProcBegin)) in H7. rewrite map_nth in H7.
+        unfold ext_mailbox1 in H7. rewrite combine_nth in H7.
+        2: { rewrite H.(wf_queue_len). now setoid_rewrite H.(wf_procs_len). }
+        rewrite <- H1, Heqp, Heqo in H7. injection H7 as ->.
+        unfold noop_msg in Heqb. apply Nat.ltb_lt in Heqb.
+        pose proof max_id_correct as [_ ?].
+        destruct (Nat.eq_dec (proj1_sig (Fin.to_nat (next_id v))) im).
+        --rewrite e0 in Heqb. unfold max in Heqb. lia.
+        --apply H7 in n1. unfold max, pid, im in Heqb. lia.
+    + apply ktrans_proc_loop_some_inv with (m := m) in H3 as (? & -> & ->); auto.
+      cbn. right. rewrite H1, Nat.eqb_refl.
+      unfold handle_recv. cbn.
+      destruct (snd s_queue0). 2: right; left.
+      left. destruct (Nat.eq_dec (fst s_queue0) 0).
+      2: destruct (fst s_queue0); lia.
+      destruct (Nat.eq_dec i n).
+      * subst. rewrite Nat.sub_diag in *.
+        apply wf_src_progress in H as ?. cbn in H5.
+        rewrite H1, Nat.add_0_r, Nat.mod_small in Heqp; [| apply max_id_correct].
+        now rewrite (proj1 (proj1 H5)) in Heqp.
+      * apply next_msg_head in H as ?; auto.
+        2: { cbn. intro. injection H5. lia. }
+        cbn in H5.
+Abort.
+
 (* Stability of variant when an uninteresting process is scheduled *)
+(* FIXME the ProcWaiting and ProcProcessing cases are duplicated. *)
+Theorem election_cst_candidates :
+  forall i (Hi : i <> 0 /\ i <= n) v T st st' qs qs',
+  election_invariant v qs st ->
+  fst (election_variant st) = n + i ->
+  proj1_sig (Fin.to_nat (next_id v)) <> (im + (n - i)) mod n ->
+  ktrans (sched v, (qs, st)) (T, (qs', st')) -> election_variant st' = election_variant st.
+Proof.
+  intros.
+  destruct st as [? [] ]; cbn in H0.
+  2: { destruct H. destruct wf_progress0 as (_ & _ & [? _]). lia. }
+  unshelve eapply election_does_progress in H as ?; eauto.
+  2: { cbn. intro. inversion H3. lia. }
+  destruct H3 as (? & ? & ?).
+  eapply sched_correct_ktrans in H2 as ?; eauto. destruct H4 as (? & ? & ?). subs.
+  apply election_map_proc_state with (Hi := proj2_sig (Fin.to_nat (next_id v))) in H as ?. red in H5. cbn in H5.
+  destruct (nth (proj1_sig (Fin.to_nat (next_id v))) s_procs0 ProcBegin) eqn:?.
+  - (* ProcBegin *)
+    eapply ktrans_proc_begin_inv with (Hi := proj2_sig (Fin.to_nat (next_id v))) in H as ?.
+    3: eauto.
+    3: rewrite Fin.of_nat_to_nat_inv; apply H4.
+    2: { cbn. intro. apply H1. rewrite H6. apply Nat.mod_wd; auto. lia. }
+    destruct H6 as (? & -> & ->). cbn. reflexivity.
+  - (* ProcWaiting *)
+    rewrite Fin.of_nat_to_nat_inv in H5. rewrite H5 in H4.
+    destruct (List.hd_error (List.nth (proj1_sig (Fin.to_nat (next_id v))) qs []%list)) eqn:?.
+    (* empty mailbox *)
+    2: now apply ktrans_proc_loop_none_inv in H4 as (? & -> & ->).
+    (* non-empty mailbox *)
+    destruct (noop_msg (proj1_sig (Fin.to_nat (next_id v))) m) eqn:?.
+    + apply ktrans_proc_loop_some_noop_inv with (m := m) in H4 as (? & -> & ->); auto.
+      cbn. f_equal. destruct (_ =? _) eqn:?; auto.
+      apply Nat.eqb_eq in Heqb0. cbn in Heqb0. subst. rewrite Heqb0 in H1.
+      clear -H0 H1 Hi. exfalso. apply H1. apply Nat.mod_wd; auto. lia.
+    + apply ktrans_proc_loop_some_inv with (m := m) in H4 as (? & -> & ->); auto.
+      cbn. f_equal. destruct (_ =? _) eqn:?; auto.
+      apply Nat.eqb_eq in Heqb0. cbn in Heqb0. cbn in H0. subst. rewrite Heqb0 in H1.
+      clear -H0 H1 Hi. exfalso. apply H1. apply Nat.mod_wd; auto. lia.
+  - (* ProcProcessing *)
+    rewrite Fin.of_nat_to_nat_inv in H5. destruct H5. rewrite H5 in H4.
+    eapply election_processing_ext_mailbox in H as ?; eauto. 2: apply (proj2_sig (Fin.to_nat (next_id v))).
+    apply hd_error_in in H7. eapply election_other_messages in H7; eauto.
+    2: { cbn in H0 |- *. intro. apply H1. rewrite H8. apply Nat.mod_wd; auto. lia. }
+    destruct H7 as (? & ? & ? & ->).
+    epose proof (H.(wf_src_candidates) (proj2_sig (Fin.to_nat (next_id v)))).
+    cbn in H9. rewrite Heqp in H9. red in H9. unfold noop_msg in H9. rewrite Nat.ltb_ge in H9.
+    destruct H9. apply Nat.le_lteq in H10 as [].
+    + eapply ktrans_proc_handle_other_candidate_gt_inv with (Hi := proj2_sig (Fin.to_nat (next_id v))) in H4 as (? & ? & ->); eauto.
+      2: { cbn in H0 |- *. intro. apply H1. rewrite H11. apply Nat.mod_wd; auto. lia. }
+      cbn. unfold election_variant.
+      cbn. apply ids_wf in H8. apply Nat.eqb_neq in H8.
+      unfold max, pid. rewrite H8. reflexivity.
+    + apply pid_inj in H10; auto.
+      2: apply (proj2_sig (Fin.to_nat (next_id v))).
+      exfalso. subst.
+      eapply election_processing_ext_mailbox in H as ?; eauto. apply hd_error_in in H10.
+      pose proof H.(wf_candidates). destruct H11 as (_ & _ & ?).
+      specialize (H11 _ (proj2_sig (Fin.to_nat (next_id v)))).
+      eapply proc_handle_msg_candidate_nonmax_inv in H9; eauto.
+      destruct H9 as (? & ? & _).
+      rewrite H9 in H11. apply H11 in H8 as ?; auto.
+      apply from_succ_absurd in H12; auto. now apply Nat.mod_upper_bound.
+  - (* ProcElected *)
+    apply wf_src_progress in H. cbn in H. now apply H in Heqp.
+Qed.
+
 Theorem election_cst_elected :
   forall i (Hi : i <> 0 /\ i < n) v T st st' qs qs',
   election_invariant v qs st ->
@@ -789,19 +1180,42 @@ Proof.
     + (* ProcWaiting *)
       rewrite H5 in H6. red in H6. rewrite H6 in H4.
       destruct (List.hd_error (List.nth (proj1_sig (Fin.to_nat (next_id v))) qs []%list)) eqn:?.
-      * (* non-empty mailbox *)
-        apply ktrans_proc_loop_some_inv with (m := m) in H4 as (? & -> & ->); auto.
+      (* empty mailbox *)
+      2: now apply ktrans_proc_loop_none_inv in H4 as (? & -> & ->).
+      (* non-empty mailbox *)
+      destruct (noop_msg (proj1_sig (Fin.to_nat (next_id v))) m) eqn:?.
+      * apply ktrans_proc_loop_some_noop_inv with (m := m) in H4 as (? & -> & ->); auto.
         cbn. f_equal. destruct (_ =? _) eqn:?; auto.
-        apply Nat.eqb_eq in Heqb. cbn in Heqb. cbn in H0. subst. rewrite Heqb in H1.
+        apply Nat.eqb_eq in Heqb0. cbn in Heqb0. cbn in H0. subst. rewrite Heqb0 in H1.
         clear -H1 Hi. exfalso. apply H1. apply Nat.mod_wd; auto. lia.
-      * (* empty mailbox *)
-        now apply ktrans_proc_loop_none_inv in H4 as (? & -> & ->).
+      * apply ktrans_proc_loop_some_inv with (m := m) in H4 as (? & -> & ->); auto.
+        cbn. f_equal. destruct (_ =? _) eqn:?; auto.
+        apply Nat.eqb_eq in Heqb0. cbn in Heqb0. cbn in H0. subst. rewrite Heqb0 in H1.
+        clear -H1 Hi. exfalso. apply H1. apply Nat.mod_wd; auto. lia.
     + (* ProcProcessing *)
-      rewrite H5 in H6. red in H6. rewrite H6 in H4.
-      eapply election_processing_ext_mailbox in H5; eauto. 2: apply (proj2_sig (Fin.to_nat (next_id v))).
-      apply hd_error_in in H5. eapply election_other_messages in H5; eauto.
-      2: { cbn in H0 |- *. intro. apply H1. rewrite H7. apply Nat.mod_wd; auto. lia. }
-      destruct H5 as (? & ? & ->).
-Abort.
+      rewrite H5 in H6. red in H6. destruct H6 as [? _]. rewrite H6 in H4.
+      eapply election_processing_ext_mailbox in H5 as ?; eauto. 2: apply (proj2_sig (Fin.to_nat (next_id v))).
+      apply hd_error_in in H7. eapply election_other_messages in H7; eauto.
+      2: { cbn in H0 |- *. intro. apply H1. rewrite H8. apply Nat.mod_wd; auto. lia. }
+      destruct H7 as (? & ? & ? & ->).
+      epose proof (H.(wf_src_candidates) (proj2_sig (Fin.to_nat (next_id v)))).
+      rewrite H5 in H9. red in H9. unfold noop_msg in H9. rewrite Nat.ltb_ge in H9.
+      destruct H9. apply Nat.le_lteq in H10 as [].
+      * eapply ktrans_proc_handle_other_candidate_gt_inv with (Hi := proj2_sig (Fin.to_nat (next_id v))) in H4 as (? & ? & ->); eauto.
+        2: { cbn in H0 |- *. intro. apply H1. rewrite H11. apply Nat.mod_wd; auto. lia. }
+        cbn. unfold election_variant.
+        cbn. apply ids_wf in H8. apply Nat.eqb_neq in H8.
+        unfold max, pid. rewrite H8. reflexivity.
+      * apply pid_inj in H10; auto.
+        2: apply (proj2_sig (Fin.to_nat (next_id v))).
+        exfalso. subst.
+        eapply election_processing_ext_mailbox in H5; eauto. apply hd_error_in in H5.
+        pose proof H.(wf_candidates). destruct H0 as (_ & _ & ?).
+        specialize (H0 _ (proj2_sig (Fin.to_nat (next_id v)))).
+        eapply proc_handle_msg_candidate_nonmax_inv in H9; eauto.
+        destruct H9 as (? & ? & _).
+        rewrite H9 in H0. apply H0 in H8 as ?; auto.
+        apply from_succ_absurd in H10; auto. now apply Nat.mod_upper_bound.
+Qed.
 
 End Election.
